Tests/FFI.lean
@@ -1,5 +1,7 @@
 import LSpec
-import YatimaStdLib.FFI.UIntByteArray
+import YatimaStdLib.UInt
+import YatimaStdLib.ByteArray
+import YatimaStdLib.ByteVector
 
 open LSpec
 
@@ -15,29 +17,58 @@ def nats : List Nat := [
   let u32 : UInt32 := .ofNat n
   let u64 : UInt64 := .ofNat n
   tSeq ++
-    (test s!"{n}₁₆ roundtrips" $ UInt16.ofByteArrayC u16.toByteArrayC == u16) ++
-    (test s!"{n}₃₂ roundtrips" $ UInt32.ofByteArrayC u32.toByteArrayC == u32) ++
-    (test s!"{n}₆₄ roundtrips" $ UInt64.ofByteArrayC u64.toByteArrayC == u64)
+    (test s!"C/Lean match for {u16}₁₆" $
+      u16.toByteArray.data == u16.toByteArrayC.data) ++
+    (test s!"C/Lean match for {u32}₃₂" $
+      u32.toByteArray.data == u32.toByteArrayC.data) ++
+    (test s!"C/Lean match for {u64}₆₄" $
+      u64.toByteArray.data == u64.toByteArrayC.data)
+
+#lspec nats.foldl (init := .done) fun tSeq n =>
+  let u16 : UInt16 := .ofNat n
+  let u32 : UInt32 := .ofNat n
+  let u64 : UInt64 := .ofNat n
+  let x  : ByteVector 2 := ⟨u16.toByteArray, UInt16.toByteArray_size_2⟩
+  let y  : ByteVector 4 := ⟨u32.toByteArray, UInt32.toByteArray_size_4⟩
+  let z  : ByteVector 8 := ⟨u64.toByteArray, UInt64.toByteArray_size_8⟩
+  tSeq ++
+    (test s!"{n}₁₆ roundtrips" $ x.toUInt16 == u16) ++
+    (test s!"{n}₃₂ roundtrips" $ y.toUInt32 == u32) ++
+    (test s!"{n}₆₄ roundtrips" $ z.toUInt64 == u64)
 
 def arrays : List ByteArray := [
   ⟨#[]⟩, ⟨#[1]⟩, ⟨#[0, 3]⟩, ⟨#[1, 1, 1]⟩, ⟨#[3, 3, 3, 3]⟩, ⟨#[13]⟩
 ]
 
 #lspec arrays.zip arrays |>.foldl (init := .done) fun tSeq (x, y) =>
-  tSeq ++ (test s!"{x} = {y}" $ x.beqC y)
+  tSeq ++ (test s!"{x} = {y}" $ x.beq y && x.beqC y)
 
 #lspec arrays.zip arrays |>.foldl (init := .done) fun tSeq (x, y) =>
-  tSeq ++ (test s!"{x} = {y}" $ x.ordC y == .eq)
+  tSeq ++ (test s!"{x} = {y}" $ x.ord y == .eq && x.ordC y == .eq)
 
 #lspec arrays.zip arrays.reverse |>.foldl (init := .done) fun tSeq (x, y) =>
-  tSeq ++ (test s!"{x} ≠ {y}" $ !x.beqC y)
+  tSeq ++ (test s!"{x} ≠ {y}" $ !x.beq y && !x.beqC y)
 
 def arrays' : List ByteArray := [
   ⟨#[1]⟩, ⟨#[2]⟩, ⟨#[0, 3, 0]⟩, ⟨#[1, 2, 1]⟩, ⟨#[3, 3, 4, 3]⟩, ⟨#[13, 0]⟩
 ]
 
 #lspec arrays.zip arrays' |>.foldl (init := .done) fun tSeq (x, y) =>
-  tSeq ++ (test s!"{x} < {y}" $ x.ordC y == .lt)
+  tSeq ++ (test s!"{x} < {y}" $ x.ord y == .lt && x.ordC y == .lt)
 
 #lspec arrays'.zip arrays |>.foldl (init := .done) fun tSeq (x, y) =>
-  tSeq ++ (test s!"{x} > {y}" $ x.ordC y == .gt)
+  tSeq ++ (test s!"{x} > {y}" $ x.ord y == .gt && x.ordC y == .gt)
+
+def sliceInputs : List (Nat × Nat) := [
+  (0, 0), (0, 1), (0, 2), (0, 3), (0, 4), (0, 5), (0, 6),
+  (1, 0), (1, 1), (1, 2), (1, 3), (1, 4), (1, 5), (1, 6),
+  (2, 0), (2, 1), (2, 2), (2, 3), (2, 4), (2, 5), (2, 6),
+  (3, 0), (3, 1), (3, 2), (3, 3), (3, 4), (3, 5), (3, 6),
+  (5, 0), (5, 1), (5, 2), (5, 3), (5, 4), (5, 5), (5, 6),
+  (6, 0), (6, 1), (6, 2), (6, 3), (6, 4), (6, 5), (6, 6)
+]
+
+#lspec arrays.foldl (init := .done) fun tSeq arr =>
+  sliceInputs.foldl (init := tSeq) fun tSeq (i, n) =>
+    tSeq ++ test s!"Lean/C match for {arr} sliced {i} {n}"
+      (arr.sliceL i n == arr.sliceC i n)
